fixing vector unfolding bug ... a bit delicate

src/ocaml-output/FSharp_Format.ml
@@ -14,43 +14,43 @@ let break0 = (break_ 0)
 
 let break1 = (text " ")
 
-let enclose = (fun _497161 _497163 _497165 -> (match ((_497161, _497163, _497165)) with
+let enclose = (fun _497171 _497173 _497175 -> (match ((_497171, _497173, _497175)) with
 | (Doc (l), Doc (r), Doc (x)) -> begin
 Doc ((Support.String.strcat (Support.String.strcat l x) r))
 end))
 
-let brackets = (fun _497167 -> (match (_497167) with
+let brackets = (fun _497177 -> (match (_497177) with
 | Doc (d) -> begin
 (enclose (text "[") (text "]") (Doc (d)))
 end))
 
-let cbrackets = (fun _497169 -> (match (_497169) with
+let cbrackets = (fun _497179 -> (match (_497179) with
 | Doc (d) -> begin
 (enclose (text "{") (text "}") (Doc (d)))
 end))
 
-let parens = (fun _497171 -> (match (_497171) with
+let parens = (fun _497181 -> (match (_497181) with
 | Doc (d) -> begin
 (enclose (text "(") (text ")") (Doc (d)))
 end))
 
-let cat = (fun _497173 _497175 -> (match ((_497173, _497175)) with
+let cat = (fun _497183 _497185 -> (match ((_497183, _497185)) with
 | (Doc (d1), Doc (d2)) -> begin
 Doc ((Support.String.strcat d1 d2))
 end))
 
 let reduce = (fun docs -> (Support.List.fold_left cat empty docs))
 
-let group = (fun _497178 -> (match (_497178) with
+let group = (fun _497188 -> (match (_497188) with
 | Doc (d) -> begin
 Doc (d)
 end))
 
 let groups = (fun docs -> (group (reduce docs)))
 
-let combine = (fun _497181 docs -> (match (_497181) with
+let combine = (fun _497191 docs -> (match (_497191) with
 | Doc (sep) -> begin
-(let select = (fun _497185 -> (match (_497185) with
+(let select = (fun _497195 -> (match (_497195) with
 | Doc (d) -> begin
 if (d = "") then begin
 None
@@ -66,20 +66,20 @@ let cat1 = (fun d1 d2 -> (reduce ((d1)::(break1)::(d2)::[])))
 
 let reduce1 = (fun docs -> (combine break1 docs))
 
-let nest = (fun i _497192 -> (match (_497192) with
+let nest = (fun i _497202 -> (match (_497202) with
 | Doc (d) -> begin
 Doc (d)
 end))
 
-let align = (fun docs -> (let _497195 = (combine hardline docs)
-in (match (_497195) with
+let align = (fun docs -> (let _497205 = (combine hardline docs)
+in (match (_497205) with
 | Doc (doc) -> begin
 Doc (doc)
 end)))
 
 let hbox = (fun d -> d)
 
-let pretty = (fun sz _497199 -> (match (_497199) with
+let pretty = (fun sz _497209 -> (match (_497209) with
 | Doc (doc) -> begin
 doc
 end))
