src/ocaml-output/Microsoft_FStar_FStar.ml
@@ -1,9 +1,9 @@
 
-let process_args = (fun _529459 -> (match (_529459) with
+let process_args = (fun _529469 -> (match (_529469) with
 | () -> begin
 (let file_list = (Support.Microsoft.FStar.Util.mk_ref [])
 in (let res = (Support.Microsoft.FStar.Getopt.parse_cmdline (Microsoft_FStar_Options.specs ()) (fun i -> (file_list := (Support.List.append (! (file_list)) ((i)::[])))))
-in (let _529466 = (match (res) with
+in (let _529476 = (match (res) with
 | Support.Microsoft.FStar.Getopt.GoOn -> begin
 (Support.Prims.ignore (Microsoft_FStar_Options.set_fstar_home ()))
 end
@@ -13,14 +13,14 @@ end)
 in (res, (! (file_list))))))
 end))
 
-let cleanup = (fun _529468 -> (match (_529468) with
+let cleanup = (fun _529478 -> (match (_529478) with
 | () -> begin
 (Support.Microsoft.FStar.Util.kill_all ())
 end))
 
 let has_prims_cache = (fun l -> (Support.List.mem "Prims.cache" l))
 
-let tc_prims = (fun _529470 -> (match (_529470) with
+let tc_prims = (fun _529480 -> (match (_529480) with
 | () -> begin
 (let solver = if (! (Microsoft_FStar_Options.verify)) then begin
 Microsoft_FStar_ToSMT_Encode.solver
@@ -28,13 +28,13 @@ end else begin
 Microsoft_FStar_ToSMT_Encode.dummy
 end
 in (let env = (Microsoft_FStar_Tc_Env.initial_env solver Microsoft_FStar_Absyn_Const.prims_lid)
-in (let _529473 = (env.Microsoft_FStar_Tc_Env.solver.Microsoft_FStar_Tc_Env.init env)
+in (let _529483 = (env.Microsoft_FStar_Tc_Env.solver.Microsoft_FStar_Tc_Env.init env)
 in (let p = (Microsoft_FStar_Options.prims ())
-in (let _529478 = (Microsoft_FStar_Parser_Driver.parse_file (Microsoft_FStar_Parser_DesugarEnv.empty_env ()) p)
-in (match (_529478) with
+in (let _529488 = (Microsoft_FStar_Parser_Driver.parse_file (Microsoft_FStar_Parser_DesugarEnv.empty_env ()) p)
+in (match (_529488) with
 | (dsenv, prims_mod) -> begin
-(let _529481 = (Microsoft_FStar_Tc_Tc.check_module env (Support.List.hd prims_mod))
-in (match (_529481) with
+(let _529491 = (Microsoft_FStar_Tc_Tc.check_module env (Support.List.hd prims_mod))
+in (match (_529491) with
 | (prims_mod, env) -> begin
 (prims_mod, dsenv, env)
 end))
@@ -49,28 +49,28 @@ end
 n
 end)
 in if (errs > 0) then begin
-(let _529487 = (Support.Microsoft.FStar.Util.fprint1 "Error: %s errors were reported (see above)\n" (Support.Microsoft.FStar.Util.string_of_int errs))
+(let _529497 = (Support.Microsoft.FStar.Util.fprint1 "Error: %s errors were reported (see above)\n" (Support.Microsoft.FStar.Util.string_of_int errs))
 in (exit (1)))
 end))
 
-let tc_one_file = (fun dsenv env fn -> (let _529494 = (Microsoft_FStar_Parser_Driver.parse_file dsenv fn)
-in (match (_529494) with
+let tc_one_file = (fun dsenv env fn -> (let _529504 = (Microsoft_FStar_Parser_Driver.parse_file dsenv fn)
+in (match (_529504) with
 | (dsenv, fmods) -> begin
-(let _529504 = ((Support.List.fold_left (fun _529497 m -> (match (_529497) with
+(let _529514 = ((Support.List.fold_left (fun _529507 m -> (match (_529507) with
 | (env, all_mods) -> begin
-(let _529501 = (Microsoft_FStar_Tc_Tc.check_module env m)
-in (match (_529501) with
+(let _529511 = (Microsoft_FStar_Tc_Tc.check_module env m)
+in (match (_529511) with
 | (ms, env) -> begin
 (env, ms)
 end))
 end)) (env, [])) fmods)
-in (match (_529504) with
+in (match (_529514) with
 | (env, all_mods) -> begin
 (dsenv, env, (Support.List.rev all_mods))
 end))
 end)))
 
-let tc_one_fragment = (fun curmod dsenv env frag -> (Support.Prims.try_with (fun _529510 -> (match (_529510) with
+let tc_one_fragment = (fun curmod dsenv env frag -> (Support.Prims.try_with (fun _529520 -> (match (_529520) with
 | () -> begin
 (match ((Microsoft_FStar_Parser_Driver.parse_fragment curmod dsenv frag)) with
 | Support.Microsoft.FStar.Util.Inl ((dsenv, modul)) -> begin
@@ -81,8 +81,8 @@ end
 | Some (_) -> begin
 (raise (Microsoft_FStar_Absyn_Syntax.Err ("Interactive mode only supports a single module at the top-level")))
 end)
-in (let _529537 = (Microsoft_FStar_Tc_Tc.tc_partial_modul env modul)
-in (match (_529537) with
+in (let _529547 = (Microsoft_FStar_Tc_Tc.tc_partial_modul env modul)
+in (match (_529547) with
 | (modul, npds, env) -> begin
 Some ((Some ((modul, npds)), dsenv, env))
 end)))
@@ -93,20 +93,20 @@ end
 (failwith "Fragment without an enclosing module")
 end
 | Some ((modul, npds)) -> begin
-(let _529550 = (Microsoft_FStar_Tc_Tc.tc_more_partial_modul env modul decls)
-in (match (_529550) with
+(let _529560 = (Microsoft_FStar_Tc_Tc.tc_more_partial_modul env modul decls)
+in (match (_529560) with
 | (modul, npds', env) -> begin
 Some ((Some ((modul, (Support.List.append npds npds'))), dsenv, env))
 end))
 end)
 end)
-end)) (fun _529509 -> (match (_529509) with
+end)) (fun _529519 -> (match (_529519) with
 | Microsoft_FStar_Absyn_Syntax.Error ((msg, r)) -> begin
-(let _529516 = (Microsoft_FStar_Tc_Errors.add_errors env (((msg, r))::[]))
+(let _529526 = (Microsoft_FStar_Tc_Errors.add_errors env (((msg, r))::[]))
 in None)
 end
 | Microsoft_FStar_Absyn_Syntax.Err (msg) -> begin
-(let _529520 = (Microsoft_FStar_Tc_Errors.add_errors env (((msg, Microsoft_FStar_Absyn_Syntax.dummyRange))::[]))
+(let _529530 = (Microsoft_FStar_Tc_Errors.add_errors env (((msg, Microsoft_FStar_Absyn_Syntax.dummyRange))::[]))
 in None)
 end
 | e -> begin
@@ -127,18 +127,18 @@ stack_elt list
 let interactive_mode = (fun dsenv env -> (let should_log = ((! (Microsoft_FStar_Options.debug)) <> [])
 in (let log = if should_log then begin
 (let transcript = (Support.Microsoft.FStar.Util.open_file_for_writing "transcript")
-in (fun line -> (let _529562 = (Support.Microsoft.FStar.Util.append_to_file transcript line)
+in (fun line -> (let _529572 = (Support.Microsoft.FStar.Util.append_to_file transcript line)
 in (Support.Microsoft.FStar.Util.flush_file transcript))))
 end else begin
 (fun line -> ())
 end
-in (let _529568 = if (Support.Option.isSome (! (Microsoft_FStar_Options.codegen))) then begin
-(let _529566 = (Support.Microsoft.FStar.Util.print_string "Code-generation is not supported in interactive mode")
+in (let _529578 = if (Support.Option.isSome (! (Microsoft_FStar_Options.codegen))) then begin
+(let _529576 = (Support.Microsoft.FStar.Util.print_string "Code-generation is not supported in interactive mode")
 in (exit (1)))
 end
 in (let chunk = (Support.Microsoft.FStar.Util.new_string_builder ())
 in (let stdin = (Support.Microsoft.FStar.Util.open_stdin ())
-in (let rec fill_chunk = (fun _529573 -> (match (_529573) with
+in (let rec fill_chunk = (fun _529583 -> (match (_529583) with
 | () -> begin
 (let line = (match ((Support.Microsoft.FStar.Util.read_line stdin)) with
 | None -> begin
@@ -147,7 +147,7 @@ end
 | Some (l) -> begin
 l
 end)
-in (let _529578 = (log line)
+in (let _529588 = (log line)
 in (let l = (Support.Microsoft.FStar.Util.trim_string line)
 in if (Support.Microsoft.FStar.Util.starts_with l "#end") then begin
 (let responses = (match ((Support.Microsoft.FStar.Util.split l " ")) with
@@ -158,22 +158,22 @@ end
 ("ok", "fail")
 end)
 in (let str = (Support.Microsoft.FStar.Util.string_of_string_builder chunk)
-in (let _529590 = (Support.Microsoft.FStar.Util.clear_string_builder chunk)
+in (let _529600 = (Support.Microsoft.FStar.Util.clear_string_builder chunk)
 in Code ((str, responses)))))
 end else begin
 if (Support.Microsoft.FStar.Util.starts_with l "#pop") then begin
-(let _529592 = (Support.Microsoft.FStar.Util.clear_string_builder chunk)
+(let _529602 = (Support.Microsoft.FStar.Util.clear_string_builder chunk)
 in Pop (l))
 end else begin
 if (Support.Microsoft.FStar.Util.starts_with l "#push") then begin
-(let _529594 = (Support.Microsoft.FStar.Util.clear_string_builder chunk)
+(let _529604 = (Support.Microsoft.FStar.Util.clear_string_builder chunk)
 in Push (l))
 end else begin
 if (l = "#finish") then begin
 (exit (0))
 end else begin
-(let _529596 = (Support.Microsoft.FStar.Util.string_builder_append chunk line)
-in (let _529598 = (Support.Microsoft.FStar.Util.string_builder_append chunk "\n")
+(let _529606 = (Support.Microsoft.FStar.Util.string_builder_append chunk line)
+in (let _529608 = (Support.Microsoft.FStar.Util.string_builder_append chunk "\n")
 in (fill_chunk ())))
 end
 end
@@ -182,17 +182,17 @@ end)))
 end))
 in (let rec go = (fun stack curmod dsenv env -> (match ((fill_chunk ())) with
 | Pop (msg) -> begin
-(let _529607 = ((Support.Prims.ignore) (Microsoft_FStar_Tc_Env.pop env msg))
-in (let _529609 = (env.Microsoft_FStar_Tc_Env.solver.Microsoft_FStar_Tc_Env.refresh ())
-in (let _529611 = ((Support.Prims.ignore) (Microsoft_FStar_Options.reset_options ()))
-in (let _529622 = (match (stack) with
+(let _529617 = ((Support.Prims.ignore) (Microsoft_FStar_Tc_Env.pop env msg))
+in (let _529619 = (env.Microsoft_FStar_Tc_Env.solver.Microsoft_FStar_Tc_Env.refresh ())
+in (let _529621 = ((Support.Prims.ignore) (Microsoft_FStar_Options.reset_options ()))
+in (let _529632 = (match (stack) with
 | [] -> begin
 (failwith "Too many pops")
 end
 | hd::tl -> begin
 (hd, tl)
 end)
-in (match (_529622) with
+in (match (_529632) with
 | ((curmod, dsenv, env), stack) -> begin
 (go stack curmod dsenv env)
 end)))))
@@ -213,24 +213,24 @@ in (dsenv, env))))
 in (let commit_mark = (fun dsenv env -> (let dsenv = (Microsoft_FStar_Parser_DesugarEnv.commit_mark dsenv)
 in (let env = (Microsoft_FStar_Tc_Env.commit_mark env)
 in (dsenv, env))))
-in (let fail = (fun curmod dsenv_mark env_mark -> (let _529653 = ((Support.Prims.ignore) (Microsoft_FStar_Tc_Errors.report_all ()))
-in (let _529655 = (Microsoft_FStar_Tc_Errors.num_errs := 0)
-in (let _529657 = (Support.Microsoft.FStar.Util.fprint1 "%s\n" fail)
-in (let _529661 = (reset_mark dsenv_mark env_mark)
-in (match (_529661) with
+in (let fail = (fun curmod dsenv_mark env_mark -> (let _529663 = ((Support.Prims.ignore) (Microsoft_FStar_Tc_Errors.report_all ()))
+in (let _529665 = (Microsoft_FStar_Tc_Errors.num_errs := 0)
+in (let _529667 = (Support.Microsoft.FStar.Util.fprint1 "%s\n" fail)
+in (let _529671 = (reset_mark dsenv_mark env_mark)
+in (match (_529671) with
 | (dsenv, env) -> begin
 (go stack curmod dsenv env)
 end))))))
-in (let _529664 = (mark dsenv env)
-in (match (_529664) with
+in (let _529674 = (mark dsenv env)
+in (match (_529674) with
 | (dsenv_mark, env_mark) -> begin
 (let res = (tc_one_fragment curmod dsenv_mark env_mark text)
 in (match (res) with
 | Some ((curmod, dsenv, env)) -> begin
 if ((! (Microsoft_FStar_Tc_Errors.num_errs)) = 0) then begin
-(let _529671 = (Support.Microsoft.FStar.Util.fprint1 "\n%s\n" ok)
-in (let _529675 = (commit_mark dsenv env)
-in (match (_529675) with
+(let _529681 = (Support.Microsoft.FStar.Util.fprint1 "\n%s\n" ok)
+in (let _529685 = (commit_mark dsenv env)
+in (match (_529685) with
 | (dsenv, env) -> begin
 (go stack curmod dsenv env)
 end)))
@@ -245,20 +245,20 @@ end))))))
 end))
 in (go [] None dsenv env)))))))))
 
-let batch_mode_tc = (fun filenames -> (let _529682 = (tc_prims ())
-in (match (_529682) with
+let batch_mode_tc = (fun filenames -> (let _529692 = (tc_prims ())
+in (match (_529692) with
 | (prims_mod, dsenv, env) -> begin
-(let _529695 = ((Support.List.fold_left (fun _529686 f -> (match (_529686) with
+(let _529705 = ((Support.List.fold_left (fun _529696 f -> (match (_529696) with
 | (all_mods, dsenv, env) -> begin
-(let _529691 = (tc_one_file dsenv env f)
-in (match (_529691) with
+(let _529701 = (tc_one_file dsenv env f)
+in (match (_529701) with
 | (dsenv, env, ms) -> begin
 ((Support.List.append all_mods ms), dsenv, env)
 end))
 end)) (prims_mod, dsenv, env)) filenames)
-in (match (_529695) with
+in (match (_529705) with
 | (all_mods, dsenv, env) -> begin
-(let _529696 = if ((! (Microsoft_FStar_Options.interactive)) && ((Microsoft_FStar_Tc_Errors.get_err_count ()) = 0)) then begin
+(let _529706 = if ((! (Microsoft_FStar_Options.interactive)) && ((Microsoft_FStar_Tc_Errors.get_err_count ()) = 0)) then begin
 (env.Microsoft_FStar_Tc_Env.solver.Microsoft_FStar_Tc_Env.refresh ())
 end else begin
 (env.Microsoft_FStar_Tc_Env.solver.Microsoft_FStar_Tc_Env.finish ())
@@ -277,30 +277,30 @@ end else begin
 "Parsed and desugared"
 end
 end
-in (let _529701 = ((Support.List.iter (fun m -> if (Microsoft_FStar_Options.should_verify m.Microsoft_FStar_Absyn_Syntax.name.Microsoft_FStar_Absyn_Syntax.str) then begin
+in (let _529711 = ((Support.List.iter (fun m -> if (Microsoft_FStar_Options.should_verify m.Microsoft_FStar_Absyn_Syntax.name.Microsoft_FStar_Absyn_Syntax.str) then begin
 (Support.Microsoft.FStar.Util.print_string (Support.Microsoft.FStar.Util.format2 "%s module: %s\n" msg (Microsoft_FStar_Absyn_Syntax.text_of_lid m.Microsoft_FStar_Absyn_Syntax.name)))
 end)) fmods)
 in (Support.Microsoft.FStar.Util.print_string "All verification conditions discharged successfully\n")))
 end)
 
 let codegen = (fun fmods -> if ((! (Microsoft_FStar_Options.codegen)) = Some ("OCaml")) then begin
-(Support.Prims.try_with (fun _529705 -> (match (_529705) with
+(Support.Prims.try_with (fun _529715 -> (match (_529715) with
 | () -> begin
 (let mllib = (Microsoft_FStar_Backends_OCaml_ASTTrans.mlmod_of_fstars (Support.List.tail fmods))
 in (let doc = (Microsoft_FStar_Backends_OCaml_Code.doc_of_mllib mllib)
-in (Support.List.iter (fun _529719 -> (match (_529719) with
+in (Support.List.iter (fun _529729 -> (match (_529729) with
 | (n, d) -> begin
 (Support.Microsoft.FStar.Util.write_file (Microsoft_FStar_Options.prependOutputDir (Support.String.strcat n ".ml")) (FSharp_Format.pretty 120 d))
 end)) doc)))
-end)) (fun _529704 -> (match (_529704) with
+end)) (fun _529714 -> (match (_529714) with
 | Microsoft_FStar_Backends_OCaml_ASTTrans.OCamlFailure ((rg, error)) -> begin
-(let _529711 = (Support.Microsoft.FStar.Util.print_string (Support.Microsoft.FStar.Util.format2 "OCaml Backend Error: %s %s\n" (Support.Microsoft.FStar.Range.string_of_range rg) (Microsoft_FStar_Backends_OCaml_ASTTrans.string_of_error error)))
+(let _529721 = (Support.Microsoft.FStar.Util.print_string (Support.Microsoft.FStar.Util.format2 "OCaml Backend Error: %s %s\n" (Support.Microsoft.FStar.Range.string_of_range rg) (Microsoft_FStar_Backends_OCaml_ASTTrans.string_of_error error)))
 in (exit (1)))
 end)))
 end)
 
-let go = (fun _529720 -> (let _529724 = (process_args ())
-in (match (_529724) with
+let go = (fun _529730 -> (let _529734 = (process_args ())
+in (match (_529734) with
 | (res, filenames) -> begin
 (match (res) with
 | Support.Microsoft.FStar.Getopt.Help -> begin
@@ -316,46 +316,46 @@ end
 (Microsoft_FStar_Parser_Driver.read_build_config f)
 end
 | _ -> begin
-(let _529733 = (Support.Microsoft.FStar.Util.print_string "--use_build_config expects just a single file on the command line and no other arguments")
+(let _529743 = (Support.Microsoft.FStar.Util.print_string "--use_build_config expects just a single file on the command line and no other arguments")
 in (exit (1)))
 end)
 end else begin
 filenames
 end
-in (let _529739 = (batch_mode_tc filenames)
-in (match (_529739) with
+in (let _529749 = (batch_mode_tc filenames)
+in (match (_529749) with
 | (fmods, dsenv, env) -> begin
-(let _529740 = (report_errors None)
+(let _529750 = (report_errors None)
 in if (! (Microsoft_FStar_Options.interactive)) then begin
 (interactive_mode dsenv env)
 end else begin
-(let _529742 = (codegen fmods)
+(let _529752 = (codegen fmods)
 in (finished_message fmods))
 end)
 end)))
 end)
 end)))
 
-let main = (fun _529744 -> (match (_529744) with
+let main = (fun _529754 -> (match (_529754) with
 | () -> begin
-(Support.Prims.try_with (fun _529746 -> (match (_529746) with
+(Support.Prims.try_with (fun _529756 -> (match (_529756) with
 | () -> begin
-(let _529757 = (go ())
-in (let _529759 = (cleanup ())
+(let _529767 = (go ())
+in (let _529769 = (cleanup ())
 in (exit (0))))
-end)) (fun _529745 -> (match (_529745) with
+end)) (fun _529755 -> (match (_529755) with
 | e -> begin
-(let _529749 = if (Microsoft_FStar_Absyn_Util.handleable e) then begin
+(let _529759 = if (Microsoft_FStar_Absyn_Util.handleable e) then begin
 (Microsoft_FStar_Absyn_Util.handle_err false () e)
 end
-in (let _529751 = if (! (Microsoft_FStar_Options.trace_error)) then begin
+in (let _529761 = if (! (Microsoft_FStar_Options.trace_error)) then begin
 (Support.Microsoft.FStar.Util.fprint2 "\nUnexpected error\n%s\n%s\n" (Support.Microsoft.FStar.Util.message_of_exn e) (Support.Microsoft.FStar.Util.trace_of_exn e))
 end else begin
 if (not ((Microsoft_FStar_Absyn_Util.handleable e))) then begin
 (Support.Microsoft.FStar.Util.fprint1 "\nUnexpected error; please file a bug report, ideally with a minimized version of the source program that triggered the error.\n%s\n" (Support.Microsoft.FStar.Util.message_of_exn e))
 end
 end
-in (let _529753 = (cleanup ())
+in (let _529763 = (cleanup ())
 in (exit (1)))))
 end)))
 end))
