examples/low-level/vectorunfoldingbug.fst
@@ -1,30 +1,9 @@
-(*--build-config
-    options:--admit_fsi Set;
-    variables:LIB=../../lib;
-    other-files:$LIB/ext.fst $LIB/set.fsi $LIB/heap.fst $LIB/st.fst $LIB/list.fst  stack.fst listset.fst st3.fst example1.fst
-  --*)
-
 module ScopedWhile3
-open StructuredMem
-open Heap
-open Stack
-open Set
-open Prims
-open List
-open ListSet
+type vector (a:Type) (n:nat) = k:nat{k < n}-> Tot a
+type smem
+assume val refExistsInMem: #a:Type -> ref a -> smem -> Tot bool
+assume val loopkupRef : #a:Type -> r:ref a -> m:smem{refExistsInMem r m==true} -> Tot bool
 
-
-
-type vector (a:Type) (n:nat) = (k:nat{k<n}) -> Tot a
-
-
-(*type  innerLoopInv (n:nat)  (res:ref (vector bool n))
-     (m:smem) =
+type innerLoopInv (n:nat) (res:ref (vector bool n)) (m:smem) =
   refExistsInMem res m
-  /\ loopkupRef res m  = loopkupRef res m*)
-
-
-  type  innerLoopInv (n:nat)  (res:ref ((k:nat{k<n}) -> Tot bool))
-       (m:smem) =
-    refExistsInMem res m
-    /\ loopkupRef res m  = loopkupRef res m
+  /\ loopkupRef res m
